examples/unit-tests/testset.fst
@@ -31,7 +31,7 @@ let test3 _ = assert (sel (upd (upd h x 0) y 1) y = 1)
 let h1 = upd (upd h x 0) y 1
 let test5 _ = assert (equal h1 (upd (upd h y 1) x 0))
 
-val ys: set aref (* required *)
+(* val ys: set aref  ... required ... NS: Not anymore *)
 let ys = Set.singleton (Ref y)
 
 let test6 _ = assert (equal h1 (concat h1 (restrict h1 (complement ys))))
